bias = 2^(k-1) - 1;

A.  
    7.0 == 0b0111.0000...  
    M = 0b1.11  
    f = 0b0.11  
    E = 2  
    e = E + bias  
    V = 2^E * M = M << E  
                = 0b111.000...  
                = 7.0  
  
B.  
    M = 0b1.111...(n+1 bits 1)  
    f = 0b0.111...(n   bits 1)  
    E = n  
    V = 2^E * M = M << E  
                = 0b111...(n+1 bits 1)  
                = 2^(n+1) - 1  
```
    s    e      f
    0  bias+n 111...(n bits 1)
```
C.  
    least standard number  
    1 111...0(k-1 bits 1) 111...(n bits 1)  
    reciprocal  
    2^-bias / (2^-n - 2)  
    ???